Convert replicated disk example to modules.

src/Examples/ReplicatedDisk/RefinementAdequacy.v
@@ -1,5 +1,5 @@
 From iris.algebra Require Import auth gmap frac agree.
-Require Export CSL.WeakestPre CSL.Lifting CSL.Adequacy CSL.RefinementAdequacy.
+Require Export CSL.WeakestPre CSL.Lifting CSL.Adequacy CSL.RefinementIdempotenceModule.
 Require Export ReplicatedDisk.TwoDiskAPI ReplicatedDisk.WeakestPre.
 Import TwoDisk.
 Require Import Spec.Proc.
@@ -22,126 +22,39 @@ Proof. solve_inG. Qed.
 
 Import TwoDisk.
 
-Section refinement.
-  Context OpT (Λa: Layer OpT).
+Module Type twodisk_refinement_type.
+  Context (OpT: Type → Type).
+  Context (Λa: Layer OpT).
   Context (impl: LayerImpl TwoDisk.Op OpT).
+  Context (Σ: gFunctors).
   Notation compile_op := (compile_op impl).
   Notation compile_rec := (compile_rec impl).
   Notation compile_seq := (compile_seq impl).
   Notation compile := (compile impl).
   Notation recover := (recover impl).
   Notation compile_proc_seq := (compile_proc_seq impl).
-  Context `{exmachPreG Σ}.
-  Context `{cfgPreG OpT Λa Σ}.
+  Context `{CFG: cfgPreG OpT Λa Σ} `{HEX: exmachPreG Σ}.
+  Context `{INV: Adequacy.invPreG Σ}.
+  Context `{REG: inG Σ (csumR countingR (authR (optionUR (exclR unitC))))}.
   Context (crash_inner: forall {_ : @cfgG OpT Λa Σ} {_: exmachG Σ}, iProp Σ).
-  Context (exec_inner: forall {_ : @cfgG OpT Λa Σ} {_ : exmachG Σ}, iProp Σ).
+  Context (exec_inner: forall {_ : @cfgG OpT Λa Σ} {_: exmachG Σ}, iProp Σ).
   Context (crash_param: forall (_ : @cfgG OpT Λa Σ) (_ : exmachG Σ), Type).
-  Context (crash_inv: forall {H1 : @cfgG OpT Λa Σ} {H2 : exmachG Σ}, @crash_param _ _ → iProp Σ).
-  Context (crash_starter: forall {H1 : @cfgG OpT Λa Σ} {H2 : exmachG Σ}, @crash_param _ _ → iProp Σ).
+  Context (crash_inv: forall {H1 : @cfgG OpT Λa Σ} {H2 : exmachG Σ},
+              @crash_param _ H2 → iProp Σ).
+  Context (crash_starter: forall {H1 : @cfgG OpT Λa Σ} {H2 : exmachG Σ},
+              @crash_param _ H2 → iProp Σ).
   Context (exec_inv: forall {_ : @cfgG OpT Λa Σ} {_ : exmachG Σ}, iProp Σ).
 
-  Context (einv_persist: forall {H1 : @cfgG OpT Λa Σ} {H2 : exmachG Σ}, Persistent (exec_inv H1 H2)).
-  Context (cinv_persist: forall {H1 : @cfgG OpT Λa Σ} {H2 : exmachG Σ}
-            {P: crash_param _ _}, Persistent (crash_inv H1 H2 P)).
-
   Context (E: coPset).
-  Context (nameIncl: nclose sourceN ⊆ E).
-  (* TODO: we should get rid of rec_seq if we're not exploiting vertical comp anymore *)
   Context (recv: proc TwoDisk.Op unit).
-  Context (recsingle: recover = rec_singleton recv).
+  Context (init_absr: Λa.(OpState) → TwoDisk.State → Prop).
+End twodisk_refinement_type.
 
-  Context (refinement_op_triples:
-             forall {H1 H2 T1 T2} j K `{LanguageCtx OpT T1 T2 Λa K} (op: OpT T1),
-               j ⤇ K (Call op) ∗ Registered ∗ (@exec_inv H1 H2) ⊢
-                 WP compile (Call op) {{ v, j ⤇ K (Ret v) ∗ Registered }}).
+Module twodisk_refinement_definitions (eRT: twodisk_refinement_type).
+  Import eRT.
 
-  Context (exec_inv_source_ctx: ∀ {H1 H2}, exec_inv H1 H2 ⊢ source_ctx).
-
-  Lemma refinement_triples:
-             forall {H1 H2 T1 T2} j K `{LanguageCtx OpT T1 T2 Λa K} (e: proc OpT T1),
-               wf_client e →
-               j ⤇ K e ∗ Registered ∗ (@exec_inv H1 H2) ⊢
-                 WP compile e {{ v, j ⤇ K (Ret v) ∗ Registered }}.
-  Proof.
-    intros ???? j K Hctx e Hwf.
-    iIntros "(Hj&Hreg&#Hinv)".
-    iAssert (⌜∃ ea: Layer.State Λa, True⌝)%I as %[? _].
-    {
-      iDestruct (exec_inv_source_ctx with "Hinv") as ((?&?)) "#Hctx".
-      eauto.
-    }
-    assert (Inhabited (Layer.State Λa)).
-    { eexists. eauto. }
-    assert (Inhabited Λa.(OpState)).
-    { eexists. destruct x; eauto. }
-    iInduction e as [] "IH" forall (j T2 K Hctx).
-    - iApply refinement_op_triples; iFrame; eauto.
-    - wp_ret. iFrame.
-    - wp_bind.
-      iApply wp_wand_l. iSplitL ""; last first.
-      * unshelve (iApply ("IH1" $! _ _ _ (fun x => K (Bind x p2)) with "[] Hj"); try iFrame).
-        { eapply Hwf. }
-        { iPureIntro. apply comp_ctx; auto. apply _. }
-      * iIntros (?) "(Hj&Hreg)".
-        iDestruct (exec_inv_source_ctx with "Hinv") as "#Hctx".
-        iMod (ghost_step_bind_ret with "Hj []") as "Hj".
-        { set_solver+. }
-        { eauto. }
-        iApply ("IH" with "[] [] Hj Hreg"); auto.
-        { iPureIntro. eapply Hwf. }
-    - iLöb as "IHloop" forall (init Hwf).
-      iDestruct (exec_inv_source_ctx with "Hinv") as "#Hctx".
-      iMod (ghost_step_loop with "Hj []") as "Hj".
-      { set_solver+. }
-      { eauto. }
-      wp_loop.
-      iApply wp_wand_l.
-      iSplitL ""; last first.
-      * rewrite /loop1. simpl.
-        unshelve (iApply ("IH" $! _ _ _ _ (fun x => K (Bind x
-                               (fun out => match out with
-                               | ContinueOutcome x => Loop body x
-                               | DoneWithOutcome r => Ret r
-                               end))) with "[] Hj Hreg")%proc).
-        { eauto. }
-        { iPureIntro. apply comp_ctx; auto. apply _. }
-      * iIntros (out) "(Hj&Hreg)".
-        destruct out.
-        ** iNext.
-           iMod (ghost_step_bind_ret with "Hj []") as "Hj".
-           { set_solver+. }
-           { eauto. }
-           iApply ("IHloop" with "[] Hj Hreg").
-           { eauto. }
-        ** iNext.
-           iMod (ghost_step_bind_ret with "Hj []") as "Hj".
-           { set_solver+. }
-           { eauto. }
-           wp_ret. iFrame.
-   - inversion Hwf.
-   - inversion Hwf.
-   - iDestruct (exec_inv_source_ctx with "Hinv") as "#Hctx".
-     iMod (ghost_step_spawn with "Hj []") as "(Hj&Hj')".
-     { set_solver+. }
-     { eauto. }
-     iDestruct "Hj'" as (j') "Hj'".
-     iApply (wp_spawn with "Hreg [Hj'] [Hj]").
-     { iNext. iIntros "Hreg'". 
-       { wp_bind.
-         iApply (wp_wand with "[Hj' Hreg'] []").
-         { unshelve (iApply ("IH" $! _ _ _ (fun x => Bind x (fun _ => Unregister))
-                               with "[] Hj' Hreg'")).
-           { eauto. }
-           { iPureIntro. apply _. }
-         }
-         { iIntros (?) "(?&?)". iApply (wp_unregister with "[$]"). iIntros "!> ?". eauto. }
-       }
-     }
-     iIntros "!> ?". iFrame.
-  Qed.
-
-  Context (recv_triple:
-             forall {H1 H2} param,
+  Definition recv_triple_type :=
+             forall H1 H2 param,
                (@crash_inv H1 H2 param) ∗ Registered ∗ (@crash_starter H1 H2 param) ⊢
                     WP recv @ NotStuck; ⊤ {{ v, |={⊤,E}=> ∃ σ2a σ2a', source_state σ2a
                     ∗ ⌜Λa.(crash_step) σ2a (Val σ2a' tt)⌝ ∗
@@ -150,318 +63,306 @@ Section refinement.
                       exec_inner Hcfg' (ExMachG Σ Hinv' exm_mem_inG
                                                         exm_disk0_inG exm_disk1_inG exm_status_inG
                                                         tr')
-                                               }}).
+                                               }}.
 
-  Context (init_absr: Λa.(OpState) → TwoDisk.State → Prop).
-  (*
-  Context (init_wf: ∀ σ1a σ1c, init_absr σ1a σ1c → state_wf σ1c).
-   *)
-  Context (init_wf: ∀ σ1a σ1c, init_absr σ1a σ1c → σ1c = TwoDisk.init_state).
+  Definition refinement_op_triples_type :=
+             forall H1 H2 T1 T2 j K `{LanguageCtx OpT T1 T2 Λa K} (op: OpT T1),
+               j ⤇ K (Call op) ∗ Registered ∗ (@exec_inv H1 H2) ⊢
+                 WP compile (Call op) {{ v, j ⤇ K (Ret v) ∗ Registered }}.
 
-  Context (init_exec_inner: ∀ σ1a σ1c, init_absr σ1a σ1c →
+  Definition init_exec_inner_type :=
+    ∀ σ1a σ1c, init_absr σ1a σ1c →
       (∀ `{Hex: exmachG Σ} `{Hcfg: cfgG OpT Λa Σ},
           (([∗ map] i ↦ v ∈ init_zero, i m↦ v) ∗
            ([∗ map] i ↦ v ∈ init_zero, i d0↦ v) ∗
            ([∗ map] i ↦ v ∈ init_zero, i d1↦ v) ∗
-           source_ctx ∗ source_state σ1a) ={⊤}=∗ exec_inner _ _)).
+           source_ctx ∗ source_state σ1a) ={⊤}=∗ exec_inner _ _).
 
-  Context (exec_inv_preserve_crash:
-      (∀ `{Hex: exmachG Σ} `{Hcfg: cfgG OpT Λa Σ},
+  Definition exec_inv_preserve_crash_type :=
+      (∀ `(Hex: exmachG Σ) `(Hcfg: cfgG OpT Λa Σ),
           exec_inv Hcfg Hex ={⊤, E}=∗ ∀ Hmem' Hreg',
           (let Hex := ExMachG Σ (exm_invG) Hmem'
                               (exm_disk0_inG) (exm_disk1_inG) (exm_status_inG)
                               Hreg' in
-              ([∗ map] i ↦ v ∈ init_zero, i m↦ v) ={E}=∗ crash_inner Hcfg Hex))).
+              ([∗ map] i ↦ v ∈ init_zero, i m↦ v) ={E}=∗ crash_inner Hcfg Hex)).
 
-  Context (crash_inv_preserve_crash:
-      (∀ `{Hex: exmachG Σ} `{Hcfg: cfgG OpT Λa Σ} param,
+  Definition crash_inv_preserve_crash_type :=
+      (∀ `(Hex: exmachG Σ) `(Hcfg: cfgG OpT Λa Σ) param,
           crash_inv Hcfg Hex param ={⊤, E}=∗ ∀ Hmem' Hreg',
           (let Hex := ExMachG Σ (exm_invG) Hmem'
                               (exm_disk0_inG) (exm_disk1_inG) (exm_status_inG)
                               Hreg' in
-              ([∗ map] i ↦ v ∈ init_zero, i m↦ v) ={E}=∗ crash_inner Hcfg Hex))).
+              ([∗ map] i ↦ v ∈ init_zero, i m↦ v) ={E}=∗ crash_inner Hcfg Hex)).
 
-  Context (crash_inner_inv :
-      (∀ `{Hex: exmachG Σ} `{Hcfg: cfgG OpT Λa Σ},
+  Definition crash_inner_inv_type :=
+      (∀ `(Hex: exmachG Σ) `(Hcfg: cfgG OpT Λa Σ),
           (∃ Hinv, crash_inner Hcfg (ExMachG Σ Hinv (exm_mem_inG)
                                              (exm_disk0_inG) (exm_disk1_inG) (exm_status_inG)
                                              (exm_treg_inG))) ∗
-          source_ctx ={⊤}=∗ ∃ param, crash_inv Hcfg Hex param ∗ crash_starter Hcfg Hex param)).
+          source_ctx ={⊤}=∗ ∃ param, crash_inv Hcfg Hex param ∗ crash_starter Hcfg Hex param).
 
-  Context (exec_inner_inv :
-      (∀ `{Hex: exmachG Σ} `{Hcfg: cfgG OpT Λa Σ},
+  Definition exec_inner_inv_type :=
+      (∀ `(Hex: exmachG Σ) `(Hcfg: cfgG OpT Λa Σ),
           (∃ Hinv, exec_inner Hcfg (ExMachG Σ Hinv (exm_mem_inG)
                                              (exm_disk0_inG) (exm_disk1_inG) (exm_status_inG)
                                              (exm_treg_inG))) ∗
-          source_ctx ={⊤}=∗ exec_inv Hcfg Hex)).
+          source_ctx ={⊤}=∗ exec_inv Hcfg Hex).
 
-  Context (exec_inv_preserve_finish:
-      (∀ `{Hex: exmachG Σ} `{Hcfg: cfgG OpT Λa Σ},
+  Definition exec_inv_preserve_finish_type :=
+      (∀ `(Hex: exmachG Σ) `(Hcfg: cfgG OpT Λa Σ),
           AllDone -∗ exec_inv Hcfg Hex ={⊤, E}=∗ ∃ (σ2a σ2a' : Λa.(OpState)), source_state σ2a
           ∗ ⌜Λa.(finish_step) σ2a (Val σ2a' tt)⌝ ∗
           ∀ `{Hcfg': cfgG OpT Λa Σ} (Hinv': invG Σ) Hmem' Hreg',
             (let Hex := ExMachG Σ Hinv' Hmem' (exm_disk0_inG) (exm_disk1_inG) (exm_status_inG)
                                 Hreg' in
             source_ctx∗ source_state σ2a' ∗ ([∗ map] i ↦ v ∈ init_zero, i m↦ v) ={⊤}=∗
-               exec_inner Hcfg' Hex))%I).
+               exec_inner Hcfg' Hex))%I.
+
+End twodisk_refinement_definitions.
 
 
-  Lemma exmach_crash_refinement_seq {T} σ1c σ1a (es: proc_seq OpT T) :
-    init_absr σ1a σ1c →
-    wf_client_seq es →
-    ¬ proc_exec_seq Λa es (rec_singleton (Ret ())) (1, σ1a) Err →
-    ∀ σ2c res, proc_exec_seq TwoDisk.l (compile_proc_seq es)
-                                        (rec_singleton recv) (1, σ1c) (Val σ2c res) →
-    ∃ σ2a, proc_exec_seq Λa es (rec_singleton (Ret tt)) (1, σ1a) (Val σ2a res).
+Module Type twodisk_refinement_obligations (eRT: twodisk_refinement_type).
+
+  Module eRD := twodisk_refinement_definitions eRT.
+  Import eRT.
+  Import eRD.
+
+  Context (recsingle: recover = rec_singleton eRT.recv).
+
+  Context (nameIncl: nclose sourceN ⊆ eRT.E).
+  Context (einv_persist: forall {H1 : @cfgG OpT Λa eRT.Σ} {H2 : _},
+              Persistent (exec_inv H1 H2)).
+  Context (cinv_persist: forall {H1 : @cfgG OpT Λa Σ} {H2 : _}
+            {P: crash_param _ _}, Persistent (crash_inv H1 H2 P)).
+
+  Context (exec_inv_source_ctx: ∀ {H1 H2}, exec_inv H1 H2 ⊢ source_ctx).
+
+  Context (recv_triple: recv_triple_type).
+  Context (init_wf: ∀ σ1a σ1c, init_absr σ1a σ1c → σ1c = TwoDisk.init_state).
+  Context (refinement_op_triples: refinement_op_triples_type).
+  Context (init_exec_inner: init_exec_inner_type).
+  Context (exec_inv_preserve_crash: exec_inv_preserve_crash_type).
+  Context (crash_inv_preserve_crash: crash_inv_preserve_crash_type).
+  Context (exec_inner_inv: exec_inner_inv_type).
+  Context (crash_inner_inv: crash_inner_inv_type).
+  Context (exec_inv_preserve_finish : exec_inv_preserve_finish_type).
+End twodisk_refinement_obligations.
+
+Module twodisk_refinement (eRT: twodisk_refinement_type) (eRO: twodisk_refinement_obligations eRT).
+
+  Module RT <: refinement_type.
+    Import eRT.
+    Definition OpC := TwoDisk.Op.
+    Definition Λc := TwoDisk.l.
+    Definition OpT := OpT.
+    Definition Λa := Λa.
+    Definition impl := impl.
+    Definition exmachG := exmachG.
+    Definition Σ := Σ.
+    Definition CFG := CFG.
+    Definition INV := INV.
+    Definition REG := REG.
+    Definition Hinstance := @exmachG_irisG.
+    Definition Hinstance_reg := @exm_treg_inG.
+    Definition set_inv_reg Hex Hinv Hreg :=
+      ExMachG Σ Hinv (@exm_mem_inG _ Hex) (@exm_disk0_inG _ Hex) (@exm_disk1_inG _ Hex)
+              (exm_status_inG) Hreg.
+
+    Definition crash_inner := crash_inner.
+    Definition exec_inner := exec_inner.
+    Definition crash_inv := crash_inv.
+    Definition crash_param := crash_param.
+    Definition crash_starter := crash_starter.
+    Definition exec_inv := exec_inv.
+    Definition E := E.
+    Definition recv := recv.
+    Definition init_absr := init_absr.
+
+  End RT.
+
+  Module RD := refinement_definitions RT.
+
+  Import RT RD.
+
+  Module RO : refinement_obligations RT.
+    Module RD := RD.
+    Import WeakestPre.
+    Import RT RD.
+
+    Definition nameIncl := eRO.nameIncl.
+    Definition einv_persist := eRO.einv_persist.
+    Definition cinv_persist := eRO.cinv_persist.
+    Existing Instances einv_persist cinv_persist.
+    Definition recsingle := eRO.recsingle.
+    Definition refinement_op_triples := eRO.refinement_op_triples.
+    Definition exec_inv_source_ctx := eRO.exec_inv_source_ctx.
+
+
+    Lemma set_inv_reg_spec0:
+             ∀ Hex, (set_inv_reg Hex (Hinstance Σ Hex).(@iris_invG OpC (Layer.State Λc) Σ)
+                                                         (Hinstance_reg Σ Hex) = Hex).
+    Proof. destruct Hex; auto. Qed.
+
+    Lemma set_inv_reg_spec1:
+      ∀ Hex Hinv Hreg, @iris_invG _ _ _ (Hinstance _ (set_inv_reg Hex Hinv Hreg)) = Hinv.
+    Proof. trivial. Qed.
+
+    Lemma set_inv_reg_spec2:
+      ∀ Hex Hinv Hreg, Hinstance_reg _ (set_inv_reg Hex Hinv Hreg) = Hreg.
+    Proof. trivial. Qed.
+
+    Lemma set_inv_reg_spec3:
+      ∀ Hex Hinv Hinv' Hreg Hreg', set_inv_reg (set_inv_reg Hex Hinv' Hreg') Hinv Hreg =
+                       (set_inv_reg Hex Hinv Hreg).
+    Proof. trivial. Qed.
+
+    Lemma register_spec `{WeakestPre.exmachG Σ}: ∃ (Interp: OpState Λc → iProp Σ),
+                (∀ n σ, @state_interp _ _ _ (Hinstance _ _) (n, σ)
+                                     -∗ thread_count_interp n ∗ Interp σ) ∧
+                ∀ n σ, thread_count_interp n ∗ Interp σ -∗ state_interp (n, σ).
+    Proof. eexists. split; eauto using thread_reg1, thread_reg2. Qed.
+
+    (* This is just to convert from the old recv_triple style to the new one. *)
+    Lemma recv_triple : recv_triple_type.
+    Proof.
+      rewrite /recv_triple_type.
+      iIntros (???) "(#Hinv&Hreg&Hstart)".
+      iPoseProof @eRO.recv_triple as "H".
+      iSpecialize ("H" with "[$]").
+      iApply (wp_wand with "H").
+      iIntros (_) "H".
+      iMod "H" as (σ2a σ2a') "(?&%&H)".
+      iModIntro. iExists _, _. iFrame.
+      iSplitR; first by iPureIntro.
+      iIntros. rewrite /post_recv.
+      iIntros (????) "((_&Hstate)&Hthread)". iModIntro. iExists _. iFrame.
+      iIntros. iModIntro. by iMod ("H" with "[$]").
+    Qed.
+
+    Existing Instance eRT.HEX.
+    Lemma init_exec_inner : init_exec_inner_type.
+    Proof.
+      rewrite /init_exec_inner_type.
+      iIntros (σ1a σ1c Hinit ???).
+      iMod (gen_heap_strong_init (mem_state σ1c)) as (hM Hmpf_eq) "(Hmc&Hm)".
+      iMod (gen_heap_strong_init init_zero) as (hD0 Hdpf_eq0) "(Hdc0&Hd0)".
+      iMod (gen_heap_strong_init init_zero) as (hD1 Hdpf_eq1) "(Hdc1&Hd1)".
+      iMod (own_alloc (Cinl (Excl tt))) as (status_name) "Hstat".
+      { constructor. }
+      set (hStatus := {| disk_status_name := status_name; disk_status_inG := _ |}).
+      iPoseProof (eRO.init_exec_inner σ1a σ1c Hinit (ExMachG Σ _ hM hD0 hD1 hStatus _) _) as "H".
+      iModIntro. iExists (ExMachG Σ _ hM hD0 hD1 hStatus _).
+      iIntros "(Hsource1&Hsource2&Hthread)".
+      iMod ("H" with "[Hm Hd0 Hd1 Hsource1 Hsource2]") as "Hinner".
+      { iFrame.
+        rewrite !(eRO.init_wf _ _ Hinit).
+        iSplitL "Hm"; [| iSplitL "Hd0"].
+        { rewrite -Hmpf_eq. iApply mem_init_to_bigOp; auto. }
+        { rewrite -Hdpf_eq0. iApply disk0_init_to_bigOp; auto. }
+        { rewrite -Hdpf_eq1. iApply disk1_init_to_bigOp; auto. }
+      }
+      rewrite !(eRO.init_wf _ _ Hinit); auto.
+      iFrame. simpl.
+      iModIntro. iExists _, _, _. iFrame.
+      iPureIntro; repeat split_and! => //=; eauto using wf_init_zero.
+    Qed.
+
+  Lemma exec_inv_preserve_crash: exec_inv_preserve_crash_type.
   Proof.
-    rewrite /compile_proc_seq. intros Hinit Hwf_seq Hno_err σ2c0 ?.
-    unshelve (eapply wp_proc_seq_refinement_adequacy with
-                  (Λc := l)
-                  (φ := fun va vc _ _ => ⌜ va = vc ⌝%I)
-                  (E0 := E); eauto).
-    clear Hno_err.
-  iAssert (∀ invG H1 ρ, |={⊤}=>
-       ∃ hM hD0 hD1 hStat tR
-            (Hmpf_eq : hM.(@gen_heap_inG addr nat Σ nat_eq_dec nat_countable) =
-          H.(@exm_preG_disk Σ).(@gen_heap_preG_inG addr nat Σ nat_eq_dec nat_countable))
-            (Hd0pf_eq : hD0.(@gen_heap_inG addr nat Σ nat_eq_dec nat_countable) =
-          H.(@exm_preG_disk Σ).(@gen_heap_preG_inG addr nat Σ nat_eq_dec nat_countable))
-            (Hd1pf_eq : hD1.(@gen_heap_inG addr nat Σ nat_eq_dec nat_countable) =
-          H.(@exm_preG_disk Σ).(@gen_heap_preG_inG addr nat Σ nat_eq_dec nat_countable)),
-         (@ex_mach_interp _ hM hD0 hD1 hStat {| treg_name := tR; treg_counter_inG := _ |} (1, σ1c)) ∗
-         (source_ctx' (ρ, σ1a) -∗ source_state σ1a ={⊤}=∗
-         own tR (Cinl (Count (-1))) ∗
-          exec_inner H1 (ExMachG Σ invG hM hD0 hD1 hStat {| treg_name := tR; treg_counter_inG := _ |})))%I
-      as "Hpre".
-  {
-  iIntros.
-  iMod (gen_heap_strong_init (mem_state σ1c)) as (hM Hmpf_eq) "(Hmc&Hm)".
-  iMod (gen_heap_strong_init init_zero) as (hD0 Hdpf_eq0) "(Hdc0&Hd0)".
-  iMod (gen_heap_strong_init init_zero) as (hD1 Hdpf_eq1) "(Hdc1&Hd1)".
-  iMod (own_alloc (Cinl (Excl tt))) as (status_name) "Hstat".
-  { constructor. }
-  iMod (own_alloc (Cinl (Count 0))) as (tR) "Ht".
-  { constructor. }
-  set (tR' := {| treg_name := tR; treg_counter_inG := _ |}).
-  set (hStatus := {| disk_status_name := status_name; disk_status_inG := _ |}).
-  iAssert (own tR (Cinl (Count 1)) ∗ own tR (Cinl (Count (-1))))%I with "[Ht]" as "(Ht&Hreg)".
-  { rewrite /Registered -own_op Cinl_op counting_op' //=. }
-  iModIntro. iExists hM, hD0, hD1, hStatus, tR, Hmpf_eq, Hdpf_eq0, Hdpf_eq1.
-  iSplitL "Hmc Hdc0 Hdc1 Hstat Ht".
-  { iFrame. iExists _, _, _. iFrame.
-    rewrite !(init_wf _ _ Hinit) //=.
-    iFrame. clear. iPureIntro; repeat split_and! => //=; eauto using wf_init_zero.
-  }
-  iIntros.
-  iPoseProof (init_exec_inner σ1a σ1c Hinit (ExMachG Σ _ hM hD0 hD1 hStatus tR') _) as "H".
-  iMod ("H" with "[-Hreg]") as "$".
-  { iFrame.
-    rewrite !(init_wf _ _ Hinit).
-    iSplitL "Hm"; [| iSplitL "Hd0"; [| iSplitL "Hd1"]].
-    { rewrite -Hmpf_eq. iApply mem_init_to_bigOp; auto. }
-    { rewrite -Hdpf_eq0. iApply disk0_init_to_bigOp; auto. }
-    { rewrite -Hdpf_eq1. iApply disk1_init_to_bigOp; auto. }
-    iExists _. eauto.
-  }
-  iFrame; eauto.
-  }
-
-  clear Hinit.
-  iInduction es as [|es] "IH" forall (σ1a σ1c) "Hpre"; first by eauto.
-  - iSplit; first by eauto.
-  iExists (fun cfgG s => ∃ (Hex : exmachG Σ), state_interp s ∗
-            (∃ (hM: gen_heapG addr nat Σ) tr
-               (Hmpf_eq : hM.(@gen_heap_inG addr nat Σ nat_eq_dec nat_countable) =
-                          H.(@exm_preG_disk Σ).(@gen_heap_preG_inG addr nat Σ
-                                                                   nat_eq_dec nat_countable))
-               (Hdpf0_eq : (@exm_disk0_inG Σ Hex).(@gen_heap_inG addr nat Σ
-                                                               nat_eq_dec nat_countable)=
-                          H.(@exm_preG_disk Σ).(@gen_heap_preG_inG addr nat Σ
-                                                                   nat_eq_dec nat_countable))
-               (Hdpf1_eq : (@exm_disk1_inG Σ Hex).(@gen_heap_inG addr nat Σ
-                                                               nat_eq_dec nat_countable)=
-                          H.(@exm_preG_disk Σ).(@gen_heap_preG_inG addr nat Σ
-                                                                   nat_eq_dec nat_countable)) ,
-            gen_heap_ctx init_zero ∗ own tr (Cinl (Count 0)) ∗ crash_inner cfgG (ExMachG Σ _ hM (exm_disk0_inG) (exm_disk1_inG) (exm_status_inG) {| treg_name := tr; treg_counter_inG := _ |})))%I; auto.
-  iIntros (invG0 Hcfg0).
-  iMod ("Hpre" $! invG0 _ _) as (hM hD0 hD1 hStatus tr ???) "(Hstate0&H)".
-  set (tR' := {| treg_name := tr; treg_counter_inG := _ |}).
-  iExists (@ex_mach_interp _ hM hD0 hD1 hStatus tR').
-  iIntros "!> (#Hsrc&Hpt0&Hstate)".
-  iMod ("H" with "Hsrc Hstate") as "(Hreg&Hinv)".
-  iMod (exec_inner_inv (ExMachG Σ _ hM hD0 hD1 hStatus tR') _ with "[Hinv]") as "#Hinv".
-  { iSplitR ""; last by (iExists _; iFrame). iExists _. iFrame. }
-  simpl.
-  iModIntro.
-  iFrame "Hstate0".
-  iSplitL "Hpt0 Hreg".
-  {  iPoseProof (@wp_mono with "[Hpt0 Hreg]") as "H"; swap 1 2.
-     { iApply @refinement_triples. destruct (Hwf_seq) as (?&?). eauto. iFrame. iFrame "Hinv".
-       iFrame "Hreg".
-     }
-     { reflexivity. }
-     simpl. rewrite /compile_whole.
-     wp_bind.
-     iApply (wp_wand with "H [Hinv]").
-     iIntros (v) "(Hpt0&Hreg)". iFrame.
-     wp_bind.
-     iApply (@wp_wait Σ {| exm_invG := invG0;
-             exm_mem_inG := hM;
-             exm_disk0_inG := hD0;
-             exm_disk1_inG := hD1;
-             exm_status_inG := hStatus;
-             exm_treg_inG := tR' |}
-               with "Hreg").
-     iIntros "!> Hdone".
-     wp_ret. iFrame. iExists _. iFrame. iIntros (σ2c) "Hmach".
-     iMod (exec_inv_preserve_finish with "Hdone Hinv") as (σ2a σ2a') "(H&Hfina&Hfinish)".
-     iDestruct "Hfina" as %Hfina.
-     iModIntro. iExists _; iFrame; auto.
-     simpl.
-     rewrite -/wp_proc_seq_refinement.
-     iIntros (σ2c'). iIntros.
-     unshelve (iExists σ2a', _); [eauto |]; [].
-     iApply "IH".
-     { iPureIntro. destruct Hwf_seq. eauto. }
-     { iIntros.
-       iMod (gen_heap_strong_init (init_zero)) as (hM' Hmpf_eq') "(Hmc&Hm)".
-       iMod (own_alloc (Cinl (Count 0))) as (tR_fresh') "Ht".
-       { constructor. }
-       iAssert (own tR_fresh' (Cinl (Count 1))
-                    ∗ own tR_fresh' (Cinl (Count (-1))))%I with "[Ht]" as "(Ht&Hreg)".
-       { rewrite /Registered -own_op Cinl_op counting_op' //=. }
-       set (tR''' := {| treg_name := tR_fresh'; treg_counter_inG := _ |}).
-       iModIntro.
-       iExists hM'. iExists hD0, hD1, hStatus.
-       iExists tR_fresh'. unshelve (iExists _, _, _); try eauto.
-       destruct σ2c as (n&σ2c). iDestruct "Hmach" as "(?&Hmach)".
-       iFrame.
-       iSplitL ("Hmc Hmach").
-       { iClear "IH". clear -Hfinish. iDestruct "Hmach" as (mem0 disk0 disk1) "(?&?&?&?&%&%&%&%&%)".
-         iExists init_zero, disk0, disk1. iFrame.
-         inversion Hfinish. subst. rewrite /crash_fun. simpl. iFrame.
-         iPureIntro. split_and!; eauto.
-         split_and!. simpl.
-         apply wf_init_zero.
-         move: H3. rewrite /TwoDisk.disk0. auto.
-         move: H4. rewrite /TwoDisk.disk1. auto.
-       }
-       iIntros "Hctx' Hsrc'". iMod ("Hfinish" $! _ _ hM' with "[-]").
-       iSplitL "Hctx'"; first by (iExists _; iFrame). iFrame.
-       { rewrite -Hmpf_eq'. iApply (@mem_init_to_bigOp _ (ExMachG Σ _ hM' hD0 hD1 hStatus tR') with "Hm"). }
-       iFrame; eauto.
-     }
-  }
-  iSplit.
-  { iIntros (σ2c) "Hmach".
-    iMod (exec_inv_preserve_crash with "Hinv") as "Hinv_post".
-    iMod (gen_heap_strong_init (init_zero)) as (hM' Hmpf_eq') "(Hmc&Hm)".
-    iMod (own_alloc (Cinl (Count 0))) as (tR_fresh') "Ht".
-    { constructor. }
-    set (tR''' := {| treg_name := tR_fresh'; treg_counter_inG := _ |}).
-    iMod ("Hinv_post" with "[Hm]") as "Hinv'".
-    { rewrite -Hmpf_eq'. iApply @mem_init_to_bigOp; auto. }
-    iIntros. iModIntro.
-    iExists (ExMachG Σ _ hM hD0 hD1 hStatus tR'). iFrame "Hmach".
-    iExists hM', tR_fresh', Hmpf_eq', H2. iFrame.
-    eauto.
-  }
-  iClear "Hsrc".
-  iModIntro. iIntros (invG Hcfg' ?? Hcrash) "(Hinv0&#Hsrc)".
-  iDestruct "Hinv0" as (HexmachG') "(Hinterp&Hinv0)".
-  iDestruct "Hinv0" as (hM' tR_fresh' Hmpf_eq' Hmdpf_eq0' Hmdpf_eq1') "(Hmc'&Hreg&Hcrash_inner)".
-  iClear "Hinv".
-  set (tR''' := {| treg_name := tR_fresh'; treg_counter_inG := _ |}).
-  iMod (crash_inner_inv (ExMachG Σ _
-                                 hM' (exm_disk0_inG) (exm_disk1_inG) (exm_status_inG) tR''') Hcfg'
-                         with "[Hcrash_inner]") as (param) "(#Hinv&Hstarter)".
-  { iIntros. simpl. iSplitR ""; last by (iExists _; iFrame).
-    iExists ( exmachG_irisG.(@iris_invG Op _ Σ)).
-    iFrame. }
-  iModIntro.
-  iAssert (own tR_fresh' (Cinl (Count 1)) ∗ own tR_fresh' (Cinl (Count (-1))))%I
-    with "[Hreg]" as "(Ht&Hreg)".
-  { rewrite /Registered -own_op Cinl_op counting_op' //=. }
-  iExists (@ex_mach_interp Σ hM' (exm_disk0_inG) (exm_disk1_inG) (exm_status_inG) tR''').
-  iSplitL "Hinterp Ht Hmc'".
-  { (* shows ex_mach_interp is holds after crash for next gen *)
-    rewrite /ex_mach_interp'.
-    rewrite /ex_mach_interp.
-    destruct a, a0.
-    iDestruct "Hinterp" as "(?&Hinterp)".
-    iDestruct "Hinterp" as (mems disk0 disk1) "(Hmem&?&?&?&%&Hp)".
-    iDestruct "Hp" as %(Hdisks&Hwf1'&Hwf2').
-    destruct Hcrash as ([]&(?&?)&Hput&Hrest).
-    inversion Hput. inversion H5. subst.
-    inversion Hrest; subst. inversion H4. subst.
-    iSplitL "Ht".
-    { iFrame. }
-    iExists init_zero, _, _.
-    iFrame.
-    iPureIntro. split_and!.
-    * rewrite /crash_fun//=.
-    * rewrite /crash_fun//=.
-    * rewrite /crash_fun/=. split.
-      ** apply wf_init_zero.
-      ** move: Hwf2'. rewrite /TwoDisk.disk0/TwoDisk.disk1. auto.
-  }
-  iSplitL "Hinv Hreg Hstarter".
-  {
-    iPoseProof (@wp_mono with "[Hinv Hreg Hstarter IH]") as "H"; swap 1 2.
-    { iApply recv_triple. iFrame "Hstarter". iFrame. iApply "Hinv". }
-    { reflexivity. }
-    iApply (@wp_wand with "H [IH]").
-    iIntros (_) "H". iIntros (σ2c) "Hinterp".
-    iMod "H". iModIntro.
-    iDestruct "H" as (σ2a σ2a') "(Hsource&Hinner&Hfinish)".
-    iExists (1, σ2a), (1, σ2a'). iFrame.
-     rewrite -/wp_proc_seq_refinement.
-     iDestruct "Hinner" as %?.
-     iSplitL "".
-     { iPureIntro. exists tt, (1, σ2a); split; eauto. econstructor. split; eauto. eauto.
-       econstructor; eauto.
-     }
-     iApply "IH".
-     { destruct Hwf_seq. eauto. }
-     { iIntros.
-       iMod (own_alloc (Cinl (Count 0))) as (tR_fresh'') "Ht".
-       { constructor. }
-       iAssert (own tR_fresh'' (Cinl (Count 1))
-                    ∗ own tR_fresh'' (Cinl (Count (-1))))%I with "[Ht]" as "(Ht&Hreg)".
-       { rewrite /Registered -own_op Cinl_op counting_op' //=. }
-       set (tR'''' := {| treg_name := tR_fresh''; treg_counter_inG := _ |}).
-       iModIntro.
-       iExists hM'.
-       iExists (HexmachG'.(@exm_disk0_inG Σ)).
-       iExists (HexmachG'.(@exm_disk1_inG Σ)).
-       iExists (HexmachG'.(@exm_status_inG Σ)).
-       iExists tR_fresh''.
-       unshelve (iExists _, _, _); eauto.
-       destruct σ2c. iDestruct "Hinterp" as "(?&?)".
-       iFrame. iIntros. iMod ("Hfinish" with "[-]"). iSplitL ""; first by (iExists _; iFrame).
-       iFrame. eauto.
-     }
-  }
-  {
-    iIntros (σ2c) "Hmach".
-    iMod (crash_inv_preserve_crash with "Hinv") as "Hinv_post".
-    iMod (gen_heap_strong_init (init_zero)) as (hM'' Hmpf_eq'') "(Hmc&Hm)".
-    iMod (own_alloc (Cinl (Count 0))) as (tR_fresh'') "Ht".
-    { constructor. }
-    set (tR'''' := {| treg_name := tR_fresh''; treg_counter_inG := _ |}).
-    iMod ("Hinv_post" with "[Hm]") as "Hinv'".
-    { rewrite -Hmpf_eq''. iApply @mem_init_to_bigOp; auto. }
-    iIntros. iModIntro.
-
-    iExists {| exm_invG := invG;
-               exm_mem_inG := hM';
-               exm_disk0_inG := HexmachG'.(@exm_disk0_inG Σ);
-               exm_disk1_inG := HexmachG'.(@exm_disk1_inG Σ);
-               exm_status_inG := HexmachG'.(@exm_status_inG Σ);
-               exm_treg_inG := tR''' |}.
-    iFrame "Hmach".
-    iFrame. unshelve (iExists hM'', tR_fresh'', Hmpf_eq'', _, _); eauto. iFrame.
-  }
+    rewrite /exec_inv_preserve_crash_type.
+    iIntros (??) "Hinv".
+    iPoseProof (eRO.exec_inv_preserve_crash with "Hinv") as "Hinv_post".
+    iMod (gen_heap_strong_init (init_zero)) as (hM Hmpf_eq) "(Hmc&Hm)".
+    iMod ("Hinv_post") as "Hinv_post".
+    iModIntro. iIntros (?).
+    iMod ("Hinv_post" with "[Hm]") as "Hinv_post".
+    { rewrite -Hmpf_eq. iApply @mem_init_to_bigOp; auto. }
+    iModIntro.
+    iIntros (n σ σ' Hcrash) "(Hmach&Hthread)".
+    iExists (ExMachG Σ (@exm_invG _ Hex) hM (@exm_disk0_inG _ Hex) (@exm_disk1_inG _ Hex)
+                     (@exm_status_inG _ Hex)
+                     (@exm_treg_inG _ Hex)).
+    iModIntro. iFrame. iDestruct "Hmach" as "(?&Hdisk)".
+    inversion Hcrash. subst.
+    iDestruct "Hdisk" as (???) "(?&?&?&?&%&%&%&%)". iFrame.
+    iSplitR ""; last done.
+    iExists _, _, _. iFrame.
+    iPureIntro; split_and!; [ auto | auto |].
+    split; [apply wf_init_zero | assumption].
   Qed.
 
-End refinement.
+  Lemma crash_inv_preserve_crash: crash_inv_preserve_crash_type.
+  Proof.
+    rewrite /crash_inv_preserve_crash_type.
+    iIntros (???) "Hinv".
+    iPoseProof (eRO.crash_inv_preserve_crash with "Hinv") as "Hinv_post".
+    iMod (gen_heap_strong_init (init_zero)) as (hM Hmpf_eq) "(Hmc&Hm)".
+    iMod ("Hinv_post") as "Hinv_post".
+    iModIntro. iIntros (?).
+    iMod ("Hinv_post" with "[Hm]") as "Hinv_post".
+    { rewrite -Hmpf_eq. iApply @mem_init_to_bigOp; auto. }
+    iModIntro.
+    iIntros (n σ σ' Hcrash) "(Hmach&Hthread)".
+    iExists (ExMachG Σ (@exm_invG _ Hex) hM (@exm_disk0_inG _ Hex) (@exm_disk1_inG _ Hex)
+                     (@exm_status_inG _ Hex)
+                     (@exm_treg_inG _ Hex)).
+    iModIntro. iFrame. iDestruct "Hmach" as "(?&Hdisk)".
+    inversion Hcrash. subst.
+    iDestruct "Hdisk" as (???) "(?&?&?&?&%&%&%&%)". iFrame.
+    iSplitR ""; last done.
+    iExists _, _, _. iFrame.
+    iPureIntro; split_and!; [ auto | auto |].
+    split; [apply wf_init_zero | assumption].
+  Qed.
+
+  Lemma state_interp_no_inv : state_interp_no_inv_type.
+  Proof. done. Qed.
+
+  Lemma crash_inner_inv : crash_inner_inv_type.
+  Proof.
+    iIntros (??) "Hinner".
+    iPoseProof (eRO.crash_inner_inv with "Hinner") as "Hinv".
+    eauto.
+  Qed.
+
+  Lemma exec_inner_inv : exec_inner_inv_type.
+  Proof.
+    iIntros (??) "Hinner".
+    iPoseProof (eRO.exec_inner_inv with "Hinner") as "Hinv".
+    eauto.
+  Qed.
+
+  Lemma exec_inv_preserve_finish : exec_inv_preserve_finish_type.
+  Proof.
+    iIntros (??) "Hdone Hinv".
+    iPoseProof (eRO.exec_inv_preserve_finish) as "H".
+    iMod ("H" $! _ _ with "[$] [$]") as (??) "(?&?&Hinv_post)".
+    iModIntro. iExists _, _. iFrame. iIntros.
+    iIntros (??? Hfinish ??) "((?&Hdisk)&?)".
+    inversion Hfinish. subst.
+    iMod (gen_heap_strong_init (init_zero)) as (hM Hmpf_eq) "(Hmc&Hm)".
+    iDestruct "Hdisk" as (???) "(_&?&?&?&%&%&%&%)". iFrame.
+    iModIntro.
+    iExists (ExMachG Σ (@exm_invG _ Hex) hM (@exm_disk0_inG _ Hex) (@exm_disk1_inG _ Hex)
+                     (@exm_status_inG _ Hex)
+                     (@exm_treg_inG _ Hex)).
+    iSplitR "Hinv_post Hm".
+    {
+      iFrame.
+      iExists init_zero, _, _. iFrame.
+      iPureIntro; split_and!; [ auto | auto |].
+      split; [apply wf_init_zero | assumption].
+    }
+    iIntros "Hstate". iSpecialize ("Hinv_post" with "[Hstate Hm]").
+    { iFrame. iDestruct "Hstate" as "(?&?)". iFrame.
+      rewrite -Hmpf_eq. iApply @mem_init_to_bigOp; auto. }
+    eauto.
+  Qed.
+  End RO.
+
+  Module R := refinement RT RO.
+
+
+  Export R.
+
+End twodisk_refinement.
